AtomicRegThm.v
@@ -1,6 +1,6 @@
 Set Implicit Arguments.
 
-Require Import AtomicReg AtomicRegIfc StoreAtomicity DataTypes.
+Require Import AtomicReg AtomicRegIfc StoreAtomicity DataTypes NamedTrans.
 
 Section ForAddr.
   Variable reqFn: Addr -> Proc -> Index -> Req.
@@ -8,19 +8,23 @@ Section ForAddr.
 
   Variable sa: StoreAtomicity reqFn respFn.
 
-  Theorem storeAtomicityImpAtomicRegBehavior n :
-    exists (al: AtomicTransList reqFn (Build_State (initData) (fun a t => 0))),
-      respFn n = getResp n al.
+  Record BehAtomicReg :=
+    { atomicBeh: AtomicTransList reqFn (Build_State (initData) (fun a t => 0));
+      respMatch: forall n, respFn n = getResp n atomicBeh
+    }.
+
+  Definition getNBeh n := getTransList (@getTransNext reqFn respFn) n.
+
+  Definition saBehAtomicReg: BehAtomicReg.
   Proof.
-    exists (buildAl reqFn respFn 0).
-    About getRespEq.
+    pose (buildAl reqFn respFn 0) as one.
+    assert (two: forall n, respFn n = getResp n one).
+    intros.
     pose proof (getRespEq sa n) as e1.
     pose proof (respEq sa n) as e2.
     rewrite <- e1 in e2.
+    fold one in e2.
     assumption.
-  Qed.
+    apply (Build_BehAtomicReg one two).
+  Defined.
 End ForAddr.
-
-Print Assumptions storeAtomicityImpAtomicRegBehavior.
-
-About storeAtomicityImpAtomicRegBehavior.
